test-suite/bugs/closed/shouldsucceed/1704.v
@@ -1,0 +1,17 @@
+
+Require Import Setoid.
+Parameter E : nat -> nat -> Prop.
+Axiom E_equiv : equiv nat E.
+Add Relation nat E
+reflexivity proved by (proj1 E_equiv)
+symmetry proved by (proj2 (proj2 E_equiv))
+transitivity proved by (proj1 (proj2 E_equiv))
+as E_rel.
+Notation "x == y" := (E x y) (at level 70, no associativity).
+Axiom r : False -> 0 == 1.
+Goal 0 == 0.
+Proof.
+rewrite r.
+refl.
+admit.
+Qed.
